---
title: "Wk 1 Discussion Post"
author: "Tyler Frankenberg"
output: html_document
---

We start with a system of 3 linear equations.

\[
\begin{align}
3x + 2y & = 1 \\
x - y & = 2 \\
4x + 2y & = 2 \\
\end{align}
\]

We'll first subtract the first from the third row, to eliminate a $y$ variable.  This gives us:

\[
\begin{align}
x - y & = 2 \\
x & = 1 \\
\end{align}
\]

We can plug our newfound value of $x$ into the other equation, which gives us:

\[
\begin{align}
1 - y & = 2 \\
\end{align}
\]

We subtract 1 from both sides to get:

\[
\begin{align}
- y & = 1 \\
\end{align}
\]

And multiply both sides by $-1$ to obtain our solution:
\[
\begin{align}
y & = -1 \\
\end{align}
\]


So, the solution to the system of linear equations

\[
\begin{align}
3x + 2y & = 1 \\
x - y & = 2 \\
4x + 2y & = 2 \\
\end{align}
\]

equals:

\[
\begin{align}
x & = 1 \\
y & = - 1
\end{align}
\]

Which we can verify by plugging our answers back in to the original system:

\[
\begin{align}
3(1) + 2(-1) & = 3 - 2 = 1 \\
1 - (-1) & = 1 + 1 = 2 \\
4(1) + 2(-1) & = 4 -2 = 2 \\
\end{align}
\]
